src/3d/TypeSizes.fst
@@ -98,6 +98,7 @@ let size_and_alignment_of_typ (env:env_t) (t:typ)
     | Pointer _ (PQ UInt64) -> Fixed 8, Some 8 //pointers are 64 bit and aligned
     | Pointer _ (PQ UInt32) -> Fixed 4, Some 4 //u32 pointers are 32 bit and aligned
     | Pointer _ _ -> failwith "Pointer sizes should already have been resolved to UInt32 or UInt64"
+    | Type_arrow _ _ -> Variable, None 
 
 let size_of_typ (env:env_t) (t:typ)
   : ML size
@@ -470,7 +471,7 @@ let decl_size_with_alignment (env:env_t) (d:decl)
 
     | Specialize _ _ _
     | ProbeFunction _ _ _ _
-    | CoerceProbeFunctionStub _ _
+    | CoerceProbeFunctionStub _ _ _
     | OutputType _
     | ExternType _
     | ExternFn _ _ _ _
